examples/counterexamples/LTL_must_pay_correct_counterexample.thy
@@ -1,0 +1,22 @@
+theory LTL_must_pay_correct_counterexample
+  imports "../coin-tea/Coin_Tea_Broken"
+begin
+
+abbreviation "Num \<equiv> value.Int"
+
+lemma LTL_must_pay_correct_counterexample :
+  "¬ (ev (state_eq (Some 2)) impl 
+    (not (label_eq ''vend'') suntil label_eq ''coin''))
+(watch drinks (
+      (STR ''init'', [])##
+      (STR ''vend'', [])##
+      (STR ''vend'', [Num 42, Num 85])##
+      (STR ''vend'', [Str ''tea''])##
+      (STR ''vend'', [Str ''tea''])##
+   trace))"
+  apply (simp add: make_full_observation_step)
+  apply (simp add: possible_steps_init init_def apply_updates_def possible_steps_vend_sufficient possible_steps_2)
+  by (simp add: ev_Stream implode_coin implode_vend suntil_Stream)
+
+
+end
