examples/counterexamples/LTL_vend_no_coin_counterexample.thy
@@ -1,0 +1,20 @@
+theory LTL_vend_no_coin_counterexample
+  imports "../coin-tea/Coin_Tea_Broken"
+begin
+
+abbreviation "Num \<equiv> value.Int"
+
+lemma LTL_vend_no_coin_counterexample :
+  "¬ (nxt (label_eq ''vend'' aand 
+    input_eq []) impl not (ev (state_eq (Some 2))))
+(watch drinks (
+      (STR ''init'', [])##
+      (STR ''vend'', [])##
+      (STR ''vend'', [Str ''tea''])##
+      (STR ''vend'', [Str ''tea'', Num 88])##
+   trace))"
+  apply (simp add: make_full_observation_step)
+  apply (simp add: possible_steps_init init_def apply_updates_def possible_steps_vend_sufficient possible_steps_2)
+  by (simp add: ev_Stream implode_coin implode_vend suntil_Stream)
+
+end
