examples/counterexamples/must_stop_to_open_false_counterexample.thy
@@ -1,0 +1,28 @@
+theory must_stop_to_open_false_counterexample
+  imports "../lift-controller/Lift_Controller_LTL"
+begin
+
+abbreviation "Num \<equiv> value.Int"
+
+lemma must_stop_to_open_false_counterexample :
+  "¬ (∀n. (alw (not (label_eq ''opendoor'' aand 
+    nxt (output_eq [Some (Str ''true''), Some (Num n)])) until 
+    label_eq ''motorstop''))
+(make_full_observation lift (Some 0) <4 $r:= Some (Num 1)> [] (
+      (STR ''continit'', [])##
+      (STR ''return'', [])##
+      (STR ''motorstop'', [Str ''true'', Str ''true''])##
+      (STR ''opendoor'', [Str ''true''])##
+      (STR ''opendoor'', [Str ''true''])##
+      (STR ''up'', [Str ''dummy__'', Num 1, Num 3, Str ''false''])##
+   trace)))"
+  apply (simp add: make_full_observation_step)
+  apply (rule_tac x=1 in exI)
+  apply (simp add: possible_steps_0 continit_def apply_updates_def return motorstop_1 One_nat_def[symmetric] opendoor_1 possible_steps_5_invalid apply_outputs_def)
+  apply (simp add: not_alw_iff)
+  apply (rule ev.step, simp, rule ev.step, simp, rule ev.step, simp)
+  apply (rule ev.base)
+  apply (rule not_until)
+   apply (simp add: nxt.simps)
+  by simp
+end
